Verify indexed priority queue only.

HOL/SepLogic/IndexedPriorityQueue.thy
@@ -1,73 +1,284 @@
 theory IndexedPriorityQueue
-imports PriorityQueue ArrayMap
+imports DynamicArray ArrayMap
 begin
 
-section {* Definitions of kv_pair and indexed_queue *}
+section {* Successor functions, eq-pred predicate *}
 
-datatype ('a, 'b) kv_pair = KVPair (key: 'a) (val: 'b)
-setup {* add_rewrite_rule_back @{thm kv_pair.collapse} *}
-setup {* add_rewrite_rule @{thm kv_pair.case} *}
-setup {* fold add_rewrite_rule @{thms kv_pair.sel} *}
+definition s1 :: "nat \<Rightarrow> nat" where "s1 m = 2 * m + 1"
+definition s2 :: "nat \<Rightarrow> nat" where "s2 m = 2 * m + 2"
 
-fun kv_pair_encode :: "('a::heap, 'b::heap) kv_pair \<Rightarrow> nat" where
-  "kv_pair_encode (KVPair k v) = to_nat (k, v)"
+theorem s_inj [forward]:
+  "s1 m = s1 m' \<Longrightarrow> m = m'" "s2 m = s2 m' \<Longrightarrow> m = m'" using s1_def s2_def by auto
+theorem s_neq [resolve]:
+  "s1 m \<noteq> s2 m'" "s1 m > m" "s2 m > m" "s2 m > s1 m" using s1_def s2_def by presburger+
+setup {* add_forward_prfstep_cond @{thm s_neq(2)} [with_term "s1 ?m"] *}
+setup {* add_forward_prfstep_cond @{thm s_neq(3)} [with_term "s2 ?m"] *}
+setup {* add_forward_prfstep_cond @{thm s_neq(4)} [with_term "s2 ?m", with_term "s1 ?m"] *}
 
-instance kv_pair :: (heap, heap) heap
-  apply (rule heap_class.intro)
-  apply (rule countable_classI [of "kv_pair_encode"])
-  apply (case_tac x, simp_all, case_tac y, simp_all)
-  ..
+inductive eq_pred :: "nat \<Rightarrow> nat \<Rightarrow> bool" where
+  "eq_pred n n"
+| "eq_pred n m \<Longrightarrow> eq_pred n (s1 m)"
+| "eq_pred n m \<Longrightarrow> eq_pred n (s2 m)"
+setup {* add_case_induct_rule @{thm eq_pred.cases} *}
+setup {* add_prop_induct_rule @{thm eq_pred.induct} *}
+setup {* add_resolve_prfstep @{thm eq_pred.intros(1)} *}
+setup {* fold add_backward_prfstep @{thms eq_pred.intros(2,3)} *}
 
-instantiation kv_pair :: (linorder, linorder) linorder begin
+theorem eq_pred_parent1 [forward]: "eq_pred i (s1 k) \<Longrightarrow> i \<noteq> s1 k \<Longrightarrow> eq_pred i k"
+@proof
+  @let "v = s1 k" @then
+  @prop_induct "eq_pred i v" "v = s1 k \<longrightarrow> i \<noteq> s1 k \<longrightarrow> eq_pred i k"
+@qed
 
-definition less: "(a < b) = (val a < val b | (val a = val b \<and> key a < key b))"
-definition less_eq: "(a \<le> b) = (val a < val b | (val a = val b \<and> key a \<le> key b))"
+theorem eq_pred_parent2 [forward]: "eq_pred i (s2 k) \<Longrightarrow> i \<noteq> s2 k \<Longrightarrow> eq_pred i k"
+@proof
+  @let "v = s2 k" @then
+  @prop_induct "eq_pred i v" "v = s2 k \<longrightarrow> i \<noteq> s2 k \<longrightarrow> eq_pred i k"
+@qed
 
-instance proof
-  fix x y z :: "('a, 'b) kv_pair"
-  show a: "(x < y) = (x \<le> y \<and> \<not> y \<le> x)"
-    using less local.less_eq by force
-  show b: "x \<le> x"
-    by (simp add: local.less_eq)
-  show c: "x \<le> y \<Longrightarrow> y \<le> z \<Longrightarrow> x \<le> z"
-    by (smt IndexedPriorityQueue.less_eq less_trans order_trans)
-  show d: "x \<le> y \<Longrightarrow> y \<le> x \<Longrightarrow> x = y"
-    using IndexedPriorityQueue.less_eq a kv_pair.expand less by fastforce
-  show e: "x \<le> y \<or> y \<le> x"
-    by (meson IndexedPriorityQueue.less_eq leI not_less_iff_gr_or_eq)
-qed end
+theorem eq_pred_cases [forward]:
+  "eq_pred i j \<Longrightarrow> \<not>eq_pred (s1 i) j \<Longrightarrow> \<not>eq_pred (s2 i) j \<Longrightarrow> j = i \<or> j = s1 i \<or> j = s2 i"
+@proof
+  @prop_induct "eq_pred i j" "\<not>eq_pred (s1 i) j \<longrightarrow> \<not>eq_pred (s2 i) j \<longrightarrow> j = i \<or> j = s1 i \<or> j = s2 i"
+@qed
 
-theorem kv_pair_less [resolve]: "KVPair k v \<le> KVPair k' v' \<Longrightarrow> v \<le> v'"
-  by (metis IndexedPriorityQueue.less_eq eq_iff kv_pair.sel(2) less_imp_le)
+theorem eq_pred_le [forward]: "eq_pred i j \<Longrightarrow> i \<le> j"
+@proof @prop_induct "eq_pred i j" "i \<le> j" @qed
+
+section {* Heap property *}
+
+(* The corresponding tree is a heap. *)
+definition is_heap :: "('a \<times> 'b::linorder) list \<Rightarrow> bool" where
+  "is_heap xs = (\<forall>i j. eq_pred i j \<longrightarrow> i < length xs \<longrightarrow> j < length xs \<longrightarrow> snd (xs ! i) \<le> snd (xs ! j))"
+setup {* add_rewrite_rule @{thm is_heap_def} *}
+
+theorem is_heap_butlast: "is_heap xs \<Longrightarrow> is_heap (butlast xs)" by auto2
+setup {* add_forward_prfstep_cond @{thm is_heap_butlast} [with_term "butlast ?xs"] *}
+
+section {* Bubble-down *}
+
+(* The corresponding tree is a heap, except k is not necessarily smaller than its descendents. *)
+definition is_heap_partial1 :: "('a \<times> 'b::linorder) list \<Rightarrow> nat \<Rightarrow> bool" where
+  "is_heap_partial1 xs k = (\<forall>i j. eq_pred i j \<longrightarrow> i < length xs \<longrightarrow> i \<noteq> k \<longrightarrow> j < length xs \<longrightarrow> snd (xs ! i) \<le> snd (xs ! j))"
+setup {* add_rewrite_rule @{thm is_heap_partial1_def} *}
+
+theorem swap_zero_is_heap_partial1:
+  "is_heap xs \<Longrightarrow> length xs > 0 \<Longrightarrow> is_heap_partial1 (butlast (list_swap xs 0 (length xs - 1))) 0"
+@proof
+  @let "xs' = list_swap xs 0 (length xs - 1)" @then
+  @have (@rule) "\<forall>i j. eq_pred i j \<longrightarrow> i < length xs - 1 \<longrightarrow> i \<noteq> 0 \<longrightarrow> j < length xs - 1 \<longrightarrow> snd (xs' ! i) \<le> snd (xs' ! j)" @with
+    @case "j = 0"
+  @end
+@qed
+setup {* add_forward_prfstep_cond @{thm swap_zero_is_heap_partial1}
+  [with_term "butlast (list_swap ?xs 0 (length ?xs - 1))"] *}
+
+theorem incr_is_heap_partial1:
+  "is_heap xs \<Longrightarrow> k < length xs \<Longrightarrow> v \<ge> snd (xs ! k) \<Longrightarrow> is_heap_partial1 (list_update xs k (fst (xs ! k), v)) k"
+@proof
+  @let "xs' = list_update xs k (fst (xs ! k), v)" @then
+  @have "\<forall>i j. eq_pred i j \<longrightarrow> i < length xs' \<longrightarrow> i \<noteq> k \<longrightarrow> j < length xs' \<longrightarrow> snd (xs' ! i) \<le> snd (xs' ! j)" @with
+    @case "j = k"
+  @end
+@qed
+setup {* add_forward_prfstep_cond @{thm incr_is_heap_partial1} [with_term "list_update ?xs ?k (fst (?xs ! ?k), ?v)"] *}
+
+(* Two cases of switching with s1 k. *)
+theorem bubble_down1:
+  "is_heap_partial1 xs k \<Longrightarrow> s2 k < length xs \<Longrightarrow> snd (xs ! (s1 k)) \<le> snd (xs ! (s2 k)) \<Longrightarrow>
+   snd (xs ! k) > snd (xs ! (s1 k)) \<Longrightarrow> is_heap_partial1 (list_swap xs k (s1 k)) (s1 k)"
+@proof
+  @let "xs' = list_swap xs k (s1 k)" @then
+  @have "\<forall>i j. eq_pred i j \<longrightarrow> i < length xs \<longrightarrow> i \<noteq> s1 k \<longrightarrow> j < length xs \<longrightarrow> snd (xs' ! i) \<le> snd (xs' ! j)" @with
+    @case "i = k" @with
+      @case "j = i" @then @case "j = s1 i" @then @case "j = s2 i" @then @case "eq_pred (s1 i) j"
+    @end
+    @case "j = k" @then @case "j = s1 k"
+  @end
+@qed
+setup {* add_forward_prfstep_cond @{thm bubble_down1} [with_term "list_swap ?xs ?k (s1 ?k)"] *}
+
+theorem bubble_down2:
+  "is_heap_partial1 xs k \<Longrightarrow> s2 k \<ge> length xs \<Longrightarrow> s1 k < length xs \<Longrightarrow> snd (xs ! k) > snd (xs ! (s1 k)) \<Longrightarrow>
+   is_heap_partial1 (list_swap xs k (s1 k)) (s1 k)"
+@proof
+  @let "xs' = list_swap xs k (s1 k)" @then
+  @have "\<forall>i j. eq_pred i j \<longrightarrow> i < length xs \<longrightarrow> i \<noteq> s1 k \<longrightarrow> j < length xs \<longrightarrow> snd (xs' ! i) \<le> snd (xs' ! j)" @with
+    @case "i = k" @with
+      @case "j = i" @then @case "j = s1 i" @then @case "j = s2 i" @then @case "eq_pred (s1 i) j"
+    @end
+    @case "j = k" @then @case "j = s1 k"
+  @end
+@qed
+setup {* add_forward_prfstep_cond @{thm bubble_down2} [with_term "list_swap ?xs ?k (s1 ?k)"] *}
+
+(* One case of switching with s2 k. *)
+theorem bubble_down3:
+  "s2 k < length xs \<Longrightarrow> snd (xs ! (s1 k)) > snd (xs ! (s2 k)) \<Longrightarrow> snd (xs ! k) > snd (xs ! (s2 k)) \<Longrightarrow>
+   is_heap_partial1 xs k \<Longrightarrow> is_heap_partial1 (list_swap xs k (s2 k)) (s2 k)"
+@proof
+  @let "xs' = list_swap xs k (s2 k)" @then
+  @have "\<forall>i j. eq_pred i j \<longrightarrow> i < length xs \<longrightarrow> i \<noteq> s2 k \<longrightarrow> j < length xs \<longrightarrow> snd (xs' ! i) \<le> snd (xs' ! j)" @with
+    @case "i = k" @with
+      @case "j = i" @then @case "j = s1 i" @then @case "j = s2 i" @then @case "eq_pred (s1 i) j"
+    @end
+    @case "j = k" @then @case "j = s2 k"
+  @end
+@qed
+setup {* add_forward_prfstep_cond @{thm bubble_down3} [with_term "list_swap ?xs ?k (s2 ?k)"] *}
+
+(* Four trivial cases. *)
+theorem bubble_down4 [forward]:
+  "is_heap_partial1 xs k \<Longrightarrow> snd (xs ! k) \<le> snd (xs ! (s1 k)) \<Longrightarrow> s2 k < length xs \<Longrightarrow>
+   snd (xs ! (s1 k)) \<le> snd (xs ! (s2 k)) \<Longrightarrow> is_heap xs"
+@proof
+  @have "\<forall>i j. eq_pred i j \<longrightarrow> i < length xs \<longrightarrow> j < length xs \<longrightarrow> snd (xs ! i) \<le> snd (xs ! j)" @with
+    @case "j = i" @then @case "j = s1 i" @then @case "j = s2 i" @then @case "eq_pred (s1 i) j"
+  @end
+@qed
+
+theorem bubble_down5 [forward]:
+  "is_heap_partial1 xs k \<Longrightarrow> snd (xs ! k) \<le> snd (xs ! (s2 k)) \<Longrightarrow> s2 k < length xs \<Longrightarrow>
+   snd (xs ! (s1 k)) > snd (xs ! (s2 k)) \<Longrightarrow> is_heap xs"
+@proof
+  @have "\<forall>i j. eq_pred i j \<longrightarrow> i < length xs \<longrightarrow> j < length xs \<longrightarrow> snd (xs ! i) \<le> snd (xs ! j)" @with
+    @case "j = i" @then @case "j = s1 i" @then @case "j = s2 i" @then @case "eq_pred (s1 i) j"
+  @end
+@qed
+
+theorem bubble_down6 [forward]:
+  "is_heap_partial1 xs k \<Longrightarrow> snd (xs ! k) \<le> snd (xs ! (s1 k)) \<Longrightarrow> s2 k \<ge> length xs \<Longrightarrow>
+   s1 k < length xs \<Longrightarrow> is_heap xs"
+@proof
+  @have "\<forall>i j. eq_pred i j \<longrightarrow> i < length xs \<longrightarrow> j < length xs \<longrightarrow> snd (xs ! i) \<le> snd (xs ! j)" @with
+    @case "j = i" @then @case "j = s1 i" @then @case "j = s2 i" @then @case "eq_pred (s1 i) j"
+  @end
+@qed
+
+theorem bubble_down7 [forward]:
+  "is_heap_partial1 xs k \<Longrightarrow> s1 k \<ge> length xs \<Longrightarrow> is_heap xs"
+@proof
+  @have "\<forall>i j. eq_pred i j \<longrightarrow> i < length xs \<longrightarrow> j < length xs \<longrightarrow> snd (xs ! i) \<le> snd (xs ! j)" @with
+    @case "j = i" @then @case "j = s1 i" @then @case "j = s2 i" @then @case "eq_pred (s1 i) j"
+  @end
+@qed
+
+setup {* del_prfstep_thm @{thm is_heap_partial1_def} *}
+
+section {* Bubble-up *}
+
+definition par :: "nat \<Rightarrow> nat" where "par m = (m - 1) div 2"
+
+theorem ps_inverse [rewrite]:
+  "par (s1 k) = k" "par (s2 k) = k" by (simp add: par_def s1_def s2_def)+
+
+theorem p_neq: "(m::nat) \<noteq> 0 \<Longrightarrow> par m < m" using par_def by auto
+setup {* add_forward_prfstep_cond @{thm p_neq} [with_term "par ?m"] *}
+
+theorem p_cases: "i \<noteq> 0 \<Longrightarrow> i = s1 (par i) \<or> i = s2 (par i)" using par_def s1_def s2_def by auto
+setup {* add_forward_prfstep_cond @{thm p_cases} [with_term "par ?m"] *}
+
+theorem eq_pred_p1: "eq_pred i j \<Longrightarrow> i \<noteq> j \<Longrightarrow> eq_pred i (par j)"
+  @proof @case_induct "eq_pred i j" @qed
+theorem eq_pred_p2: "eq_pred i j \<Longrightarrow> i \<noteq> 0 \<Longrightarrow> eq_pred (par i) j"
+  @proof @prop_induct "eq_pred i j" "i \<noteq> 0 \<longrightarrow> eq_pred (par i) j" @qed
+theorem eq_pred_p3: "i \<noteq> 0 \<Longrightarrow> eq_pred (par i) i" by auto2
+setup {* fold add_forward_prfstep [@{thm eq_pred_p1}, @{thm eq_pred_p2}] *}
+setup {* add_forward_prfstep_cond @{thm eq_pred_p3} [with_term "par ?i"] *}
+
+theorem heap_implies_hd_min [backward2]:
+  "is_heap xs \<Longrightarrow> xs \<noteq> [] \<Longrightarrow> i < length xs \<Longrightarrow> snd (hd xs) \<le> snd (xs ! i)"
+@proof
+  @strong_induct i
+  @case "i = 0" @then @apply_induct_hyp "par i"
+@qed
+
+(* The corresponding tree is a heap, except k is not necessarily greater than its ancestors. *)
+definition is_heap_partial2 :: "('a \<times> 'b::linorder) list \<Rightarrow> nat \<Rightarrow> bool" where
+  "is_heap_partial2 xs k = (\<forall>i j. eq_pred i j \<longrightarrow> i < length xs \<longrightarrow> j < length xs \<longrightarrow> j \<noteq> k \<longrightarrow> snd (xs ! i) \<le> snd (xs ! j))"
+setup {* add_rewrite_rule @{thm is_heap_partial2_def} *}
+
+theorem bubble_up1 [forward]:
+  "is_heap_partial2 xs k \<Longrightarrow> snd (xs ! k) < snd (xs ! (par k)) \<Longrightarrow> k \<noteq> 0 \<Longrightarrow> k < length xs \<Longrightarrow>
+   is_heap_partial2 (list_swap xs k (par k)) (par k)"
+@proof
+  @let "xs' = list_swap xs k (par k)" @then
+  @have "\<forall>i j. eq_pred i j \<longrightarrow> i < length xs \<longrightarrow> j < length xs \<longrightarrow> j \<noteq> par k \<longrightarrow> snd (xs' ! i) \<le> snd (xs' ! j)" @with
+    @case "j = k" @with @case "i = k" @then @case "i = par k" @end
+    @case "i = k" @then @case "i = par k"
+  @end
+@qed
+
+theorem bubble_up2 [forward]:
+  "is_heap_partial2 xs k \<Longrightarrow> snd (xs ! k) \<ge> snd (xs ! (par k)) \<Longrightarrow> k \<noteq> 0 \<Longrightarrow> k < length xs \<Longrightarrow> is_heap xs"
+@proof
+  @have "\<forall>i j. eq_pred i j \<longrightarrow> i < length xs \<longrightarrow> j < length xs \<longrightarrow> snd (xs ! i) \<le> snd (xs ! j)" @with
+    @case "j = k" @with @case "i = k" @end
+  @end
+@qed      
+
+theorem bubble_up3 [forward]: "is_heap_partial2 xs 0 \<Longrightarrow> is_heap xs" by auto2
+theorem bubble_up4 [forward]: "is_heap_partial2 xs k \<Longrightarrow> k \<ge> length xs \<Longrightarrow> is_heap xs" by auto2
+
+theorem append_is_heap_partial2:
+  "is_heap xs \<Longrightarrow> is_heap_partial2 (xs @ [x]) (length xs)" by auto2
+setup {* add_forward_prfstep_cond @{thm append_is_heap_partial2} [with_term "?xs @ [?x]"] *}
+
+theorem desc_is_heap_partial2:
+  "is_heap xs \<Longrightarrow> k < length xs \<Longrightarrow> v < snd (xs ! k) \<Longrightarrow> is_heap_partial2 (list_update xs k (fst (xs ! k), v)) k"
+@proof
+  @let "xs' = list_update xs k (fst (xs ! k), v)" @then
+  @have "\<forall>i j. eq_pred i j \<longrightarrow> i < length xs' \<longrightarrow> j < length xs' \<longrightarrow> j \<noteq> k \<longrightarrow> snd (xs' ! i) \<le> snd (xs' ! j)" @with
+    @case "i = k" @end
+@qed
+setup {* add_forward_prfstep_cond @{thm desc_is_heap_partial2} [with_term "list_update ?xs ?k (fst (?xs ! ?k), ?v)"] *}
+
+setup {* fold del_prfstep_thm [@{thm eq_pred_p1}, @{thm eq_pred_p2}, @{thm eq_pred_p3}] *}
+setup {* del_prfstep_thm @{thm p_cases} *}
+setup {* del_prfstep_thm @{thm is_heap_partial2_def} *}
+
+section {* Delete-min *}
+
+theorem mset_butlast [rewrite]: "length xs > 0 \<Longrightarrow> mset (butlast xs) = mset xs - {# last xs #}"
+  by (metis add_diff_cancel_right' append_butlast_last_id length_greater_0_conv list.size(3)
+      mset.simps(2) size_eq_0_iff_empty size_mset union_code)
+
+theorem last_swap: "length xs > 0 \<Longrightarrow> (list_swap xs 0 (length xs - 1)) ! (length xs - 1) = xs ! 0"
+  by (simp add: list_swap_eval(2))
+
+theorem last_swap' [rewrite]: "length xs > 0 \<Longrightarrow> last (list_swap xs 0 (length xs - 1)) = hd xs"
+  by (metis hd_conv_nth last_conv_nth last_swap length_swap list.size(3) not_gr0)
+    
+section {* Indexed priority queue *}
 
 datatype 'a indexed_pqueue =
-  Indexed_PQueue (pqueue: "(nat, 'a) kv_pair dynamic_array") (index: "nat array_map")
+  Indexed_PQueue (pqueue: "(nat \<times> 'a) dynamic_array") (index: "nat array_map")
 setup {* add_rewrite_rule_back @{thm indexed_pqueue.collapse} *}
 setup {* add_rewrite_rule @{thm indexed_pqueue.case} *}
 setup {* fold add_rewrite_rule @{thms indexed_pqueue.sel} *}
 
-definition index_of_pqueue :: "(nat, 'a) kv_pair list \<Rightarrow> (nat, nat) map \<Rightarrow> bool" where
+definition index_of_pqueue :: "(nat \<times> 'a) list \<Rightarrow> (nat, nat) map \<Rightarrow> bool" where
   "index_of_pqueue xs m = (
-    (\<forall>i<length xs. m\<langle>key (xs ! i)\<rangle> = Some i) \<and>
-    (\<forall>i k. m\<langle>k\<rangle> = Some i \<longrightarrow> i < length xs \<and> key (xs ! i) = k))"
+    (\<forall>i<length xs. m\<langle>fst (xs ! i)\<rangle> = Some i) \<and>
+    (\<forall>i k. m\<langle>k\<rangle> = Some i \<longrightarrow> i < length xs \<and> fst (xs ! i) = k))"
 setup {* add_rewrite_rule @{thm index_of_pqueue_def} *}
 
-definition unique_keys :: "(nat, 'a) kv_pair list \<Rightarrow> bool" where
-  "unique_keys xs = (\<forall>m n. m < length xs \<longrightarrow> n < length xs \<longrightarrow> m \<noteq> n \<longrightarrow> key (xs ! m) \<noteq> key (xs ! n))"
+definition unique_keys :: "(nat \<times> 'a) list \<Rightarrow> bool" where
+  "unique_keys xs = (\<forall>m n. m < length xs \<longrightarrow> n < length xs \<longrightarrow> m \<noteq> n \<longrightarrow> fst (xs ! m) \<noteq> fst (xs ! n))"
 setup {* add_rewrite_rule @{thm unique_keys_def} *}
 
 theorem has_index_unique_key [forward]:
   "index_of_pqueue xs m \<Longrightarrow> unique_keys xs" by auto2
 
-definition key_within_range :: "(nat, 'a) kv_pair list \<Rightarrow> nat \<Rightarrow> bool" where
-  "key_within_range xs n = (\<forall>p. p \<in># mset xs \<longrightarrow> key p < n)"
+definition key_within_range :: "(nat \<times> 'a) list \<Rightarrow> nat \<Rightarrow> bool" where
+  "key_within_range xs n = (\<forall>p. p \<in># mset xs \<longrightarrow> fst p < n)"
 setup {* add_rewrite_rule @{thm key_within_range_def} *}
 
 theorem key_within_range_on_index:
-  "key_within_range xs n \<Longrightarrow> i < length xs \<Longrightarrow> key (xs ! i) < n" by auto2
-setup {* add_forward_prfstep_cond @{thm key_within_range_on_index} [with_term "key (?xs ! ?i)"] *}
+  "key_within_range xs n \<Longrightarrow> i < length xs \<Longrightarrow> fst (xs ! i) < n" by auto2
+setup {* add_forward_prfstep_cond @{thm key_within_range_on_index} [with_term "fst (?xs ! ?i)"] *}
 
-fun idx_pqueue :: "(nat, 'a::{heap,linorder}) kv_pair list \<Rightarrow> 'a indexed_pqueue \<Rightarrow> assn" where
+fun idx_pqueue :: "(nat \<times> 'a::{heap,linorder}) list \<Rightarrow> 'a indexed_pqueue \<Rightarrow> assn" where
   "idx_pqueue xs (Indexed_PQueue pq idx) =
     (\<exists>\<^sub>Am. dyn_array xs pq * amap m idx * \<up>(index_of_pqueue xs m) * \<up>(key_within_range xs (alen idx)))"
 setup {* add_rewrite_ent_rule @{thm idx_pqueue.simps} *}
@@ -81,7 +292,7 @@ section {* Basic operations on indexed_queue *}
 
 definition idx_pqueue_empty :: "nat \<Rightarrow> 'a::heap \<Rightarrow> 'a indexed_pqueue Heap" where
   "idx_pqueue_empty k x = do {
-    pq \<leftarrow> dyn_array_new (KVPair 0 x);
+    pq \<leftarrow> dyn_array_new (0, x);
     idx \<leftarrow> amap_new k;
     return (Indexed_PQueue pq idx) }"
 declare idx_pqueue_empty_def [sep_proc_defs]
@@ -92,7 +303,7 @@ theorem index_of_pqueue_empty [resolve]:
 theorem idx_pqueue_empty_rule [hoare_triple]:
   "<emp> idx_pqueue_empty k x <\<lambda>r. idx_pqueue [] r * \<up>(alen (index r) = k)>" by auto2
 
-definition idx_pqueue_nth :: "'a::heap indexed_pqueue \<Rightarrow> nat \<Rightarrow> (nat, 'a) kv_pair Heap" where
+definition idx_pqueue_nth :: "'a::heap indexed_pqueue \<Rightarrow> nat \<Rightarrow> (nat \<times> 'a) Heap" where
   "idx_pqueue_nth p i = array_nth (pqueue p) i"
 declare idx_pqueue_nth_def [sep_proc_defs]
 
@@ -121,18 +332,18 @@ definition idx_pqueue_swap :: "'a::{heap,linorder} indexed_pqueue \<Rightarrow> 
    (case p of Indexed_PQueue pq idx \<Rightarrow> do {
       pr_i \<leftarrow> array_nth pq i;
       pr_j \<leftarrow> array_nth pq j;
-      amap_update (key pr_i) j idx;
-      amap_update (key pr_j) i idx;
+      amap_update (fst pr_i) j idx;
+      amap_update (fst pr_j) i idx;
       array_swap pq i j
     })"
 declare idx_pqueue_swap_def [sep_proc_defs]
 
 theorem index_of_pqueue_swap [backward2]:
   "index_of_pqueue xs m \<Longrightarrow> i < length xs \<Longrightarrow> j < length xs \<Longrightarrow>
-   index_of_pqueue (list_swap xs i j) (m {key (xs ! i) \<rightarrow> j} {key (xs ! j) \<rightarrow> i})"
+   index_of_pqueue (list_swap xs i j) (m {fst (xs ! i) \<rightarrow> j} {fst (xs ! j) \<rightarrow> i})"
 @proof
-  @let "m' = m {key (xs ! i) \<rightarrow> j} {key (xs ! j) \<rightarrow> i}" @then
-  @have (@rule) "\<forall>k<length xs. m'\<langle>key (list_swap xs i j ! k)\<rangle> = Some k" @with
+  @let "m' = m {fst (xs ! i) \<rightarrow> j} {fst (xs ! j) \<rightarrow> i}" @then
+  @have (@rule) "\<forall>k<length xs. m'\<langle>fst (list_swap xs i j ! k)\<rangle> = Some k" @with
     @case "k = i" @then @case "k = j"
   @end
 @qed
@@ -145,36 +356,37 @@ theorem idx_pqueue_swap_rule [hoare_triple, hoare_create_case]:
 definition idx_pqueue_push :: "nat \<Rightarrow> 'a::heap \<Rightarrow> 'a indexed_pqueue \<Rightarrow> 'a indexed_pqueue Heap" where
   "idx_pqueue_push k v p = do {
     len \<leftarrow> array_length (pqueue p);
-    d' \<leftarrow> push_array (KVPair k v) (pqueue p);
+    d' \<leftarrow> push_array (k, v) (pqueue p);
     amap_update k len (index p);
     return (Indexed_PQueue d' (index p))
    }"
 declare idx_pqueue_push_def [sep_proc_defs]
 
-definition has_key :: "(nat, 'a) kv_pair list \<Rightarrow> nat \<Rightarrow> bool" where
-  "has_key xs k = (\<exists>v'. KVPair k v' \<in># mset xs)"
+definition has_key :: "(nat \<times> 'a) list \<Rightarrow> nat \<Rightarrow> bool" where
+  "has_key xs k = (\<exists>v'. (k, v') \<in># mset xs)"
 setup {* add_rewrite_rule @{thm has_key_def} *}
 
 theorem not_has_key [forward, backward2]:
-  "\<not>(has_key xs k) \<Longrightarrow> p \<in># mset xs \<Longrightarrow> k \<noteq> key p" by auto2
+  "\<not>(has_key xs k) \<Longrightarrow> p \<in># mset xs \<Longrightarrow> k \<noteq> fst p"
+@proof @have "p = (fst p, snd p)" @qed
 
 theorem index_of_pqueue_push [backward2]:
-  "index_of_pqueue xs m \<Longrightarrow> \<not>has_key xs k \<Longrightarrow> index_of_pqueue (xs @ [KVPair k v]) (m{k \<rightarrow> length xs})"
+  "index_of_pqueue xs m \<Longrightarrow> \<not>has_key xs k \<Longrightarrow> index_of_pqueue (xs @ [(k, v)]) (m{k \<rightarrow> length xs})"
 @proof
-  @let "xs' = xs @ [KVPair k v]" @then
+  @let "xs' = xs @ [(k, v)]" @then
   @let "m' = m{k \<rightarrow> length xs}" @then
-  @have "\<forall>j<length xs'. m'\<langle>key (xs' ! j)\<rangle> = Some j" @with @case "j = length xs" @end
+  @have "\<forall>j<length xs'. m'\<langle>fst (xs' ! j)\<rangle> = Some j" @with @case "j = length xs" @end
 @qed
 
 theorem idx_pqueue_push_rule [hoare_triple]:
   "<idx_pqueue xs p * \<up>(k < alen (index p)) * \<up>(\<not>has_key xs k)>
    idx_pqueue_push k v p
-   <\<lambda>r. idx_pqueue (xs @ [KVPair k v]) r>\<^sub>t" by auto2
+   <\<lambda>r. idx_pqueue (xs @ [(k, v)]) r>\<^sub>t" by auto2
 
-definition idx_pqueue_pop :: "'a::heap indexed_pqueue \<Rightarrow> ((nat, 'a) kv_pair \<times> 'a indexed_pqueue) Heap" where
+definition idx_pqueue_pop :: "'a::heap indexed_pqueue \<Rightarrow> ((nat \<times> 'a) \<times> 'a indexed_pqueue) Heap" where
   "idx_pqueue_pop p = do {
      (x, d') \<leftarrow> pop_array (pqueue p);
-     amap_delete (key x) (index p);
+     amap_delete (fst x) (index p);
      return (x, Indexed_PQueue d' (index p))
    }"
 declare idx_pqueue_pop_def [sep_proc_defs]
@@ -186,45 +398,45 @@ theorem idx_pqueue_pop_rule [hoare_triple]:
 @proof @case "xs = []" @qed
 
 theorem index_of_pqueue_update:
-  "index_of_pqueue xs m \<Longrightarrow> m\<langle>k\<rangle> = Some i \<Longrightarrow> index_of_pqueue (list_update xs i (KVPair k v)) m"
+  "index_of_pqueue xs m \<Longrightarrow> m\<langle>k\<rangle> = Some i \<Longrightarrow> index_of_pqueue (list_update xs i (k, v)) m"
 @proof
-  @let "xs' = list_update xs i (KVPair k v)" @then
-  @have (@rule) "\<forall>j<length xs'. m\<langle>key (xs' ! j)\<rangle> = Some j" @with @case "j = i" @end
+  @let "xs' = list_update xs i (k, v)" @then
+  @have (@rule) "\<forall>j<length xs'. m\<langle>fst (xs' ! j)\<rangle> = Some j" @with @case "j = i" @end
 @qed
-setup {* add_forward_prfstep_cond @{thm index_of_pqueue_update} [with_term "list_update ?xs ?i (KVPair ?k ?v)"] *}
+setup {* add_forward_prfstep_cond @{thm index_of_pqueue_update} [with_term "list_update ?xs ?i (?k, ?v)"] *}
 
 theorem key_within_range_update [backward2]:
-  "key_within_range xs n \<Longrightarrow> i < length xs \<Longrightarrow> k < n \<Longrightarrow> key_within_range (list_update xs i (KVPair k v)) n"
+  "key_within_range xs n \<Longrightarrow> i < length xs \<Longrightarrow> k < n \<Longrightarrow> key_within_range (list_update xs i (k, v)) n"
 @proof
-  @let "xs' = list_update xs i (KVPair k v)" @then
-  @have "\<forall>p. p \<in># mset xs' \<longrightarrow> key p < n" @with
+  @let "xs' = list_update xs i (k, v)" @then
+  @have "\<forall>p. p \<in># mset xs' \<longrightarrow> fst p < n" @with
     @obtain j where "j < length xs' \<and> p = xs' ! j" @then @case "j = i"
   @end
 @qed
 
 theorem array_upd_idx_pqueue_rule [hoare_triple]:
-  "<idx_pqueue xs p * \<up>(i < length xs) * \<up>(k = key (xs ! i))>
-   array_upd i (KVPair k v) (pqueue p)
-   <\<lambda>_. idx_pqueue (list_update xs i (KVPair k v)) p>" by auto2
+  "<idx_pqueue xs p * \<up>(i < length xs) * \<up>(k = fst (xs ! i))>
+   array_upd i (k, v) (pqueue p)
+   <\<lambda>_. idx_pqueue (list_update xs i (k, v)) p>" by auto2
 
 setup {* del_prfstep_thm @{thm indexed_pqueue.collapse} *}
 
 section {* Mapping from list of kv-pairs. *}
 
-definition map_of_kv_set :: "('a, 'b) kv_pair set \<Rightarrow> ('a, 'b) map" where
-  "map_of_kv_set S = Map (\<lambda>a. THE_unique (\<lambda>b. KVPair a b \<in> S))"
+definition map_of_kv_set :: "('a \<times> 'b) set \<Rightarrow> ('a, 'b) map" where
+  "map_of_kv_set S = Map (\<lambda>a. THE_unique (\<lambda>b. (a, b) \<in> S))"
 setup {* add_rewrite_rule @{thm map_of_kv_set_def} *}
 
 setup {* add_gen_prfstep ("THE_unique_case",
-  [WithTerm @{term_pat "THE_unique (\<lambda>b. KVPair ?a b \<in> ?S)"},
-   CreateCase @{term_pat "\<exists>!b. KVPair ?a b \<in> ?S"}]) *}
+  [WithTerm @{term_pat "THE_unique (\<lambda>b. (?a, b) \<in> ?S)"},
+   CreateCase @{term_pat "\<exists>!b. (?a, b) \<in> ?S"}]) *}
 
-definition unique_keys_set :: "(nat, 'a) kv_pair set \<Rightarrow> bool" where
-  "unique_keys_set S = (\<forall>i x y. KVPair i x \<in> S \<longrightarrow> KVPair i y \<in> S \<longrightarrow> x = y)"
+definition unique_keys_set :: "(nat \<times> 'a) set \<Rightarrow> bool" where
+  "unique_keys_set S = (\<forall>i x y. (i, x) \<in> S \<longrightarrow> (i, y) \<in> S \<longrightarrow> x = y)"
 setup {* add_rewrite_rule @{thm unique_keys_set_def} *}
 
 theorem unique_keys_imp [forward]:
-  "unique_keys_set S \<Longrightarrow> KVPair i x \<in> S \<Longrightarrow> \<exists>!x. KVPair i x \<in> S" by auto2
+  "unique_keys_set S \<Longrightarrow> (i, x) \<in> S \<Longrightarrow> \<exists>!x. (i, x) \<in> S" by auto2
 
 theorem in_set_union_single: "x \<in> A \<union> {y} \<Longrightarrow> x = y \<or> x \<in> A" by auto
 setup {* add_forward_prfstep_cond @{thm in_set_union_single} [with_cond "?x \<noteq> ?y"] *}
@@ -232,30 +444,30 @@ theorem member_union_single: "x \<in> A \<union> {x}" by simp
 setup {* add_forward_prfstep_cond @{thm member_union_single} [with_term "?A \<union> {?x}"] *}
 
 theorem map_of_kv_set_insert [rewrite]:
-  "unique_keys_set T \<Longrightarrow> \<forall>v. KVPair k v \<notin> T \<Longrightarrow> map_of_kv_set (T \<union> { KVPair k v }) = (map_of_kv_set T) {k \<rightarrow> v}"
+  "unique_keys_set T \<Longrightarrow> \<forall>v. (k, v) \<notin> T \<Longrightarrow> map_of_kv_set (T \<union> { (k, v) }) = (map_of_kv_set T) {k \<rightarrow> v}"
 @proof
-  @let "S = T \<union> { KVPair k v }" @then
+  @let "S = T \<union> { (k, v) }" @then
   @have "T \<subseteq> S" @then @have "unique_keys_set S"
 @qed
 
 theorem map_of_kv_set_delete [rewrite]:
-  "unique_keys_set T \<Longrightarrow> KVPair k v \<in> T \<Longrightarrow> map_of_kv_set (T - { KVPair k v }) = delete_map k (map_of_kv_set T)"
+  "unique_keys_set T \<Longrightarrow> (k, v) \<in> T \<Longrightarrow> map_of_kv_set (T - { (k, v) }) = delete_map k (map_of_kv_set T)"
 @proof
-  @let "S = T - { KVPair k v }" @then
+  @let "S = T - { (k, v) }" @then
   @have "S \<subseteq> T" @then @have "unique_keys_set S"
 @qed
 
 theorem map_of_kv_set_update [rewrite]:
-  "unique_keys_set T \<Longrightarrow> KVPair k v \<in> T \<Longrightarrow>
-   map_of_kv_set ((T - { KVPair k v }) \<union> { KVPair k v' }) = (map_of_kv_set T) {k \<rightarrow> v'}"
+  "unique_keys_set T \<Longrightarrow> (k, v) \<in> T \<Longrightarrow>
+   map_of_kv_set ((T - { (k, v) }) \<union> { (k, v') }) = (map_of_kv_set T) {k \<rightarrow> v'}"
 @proof
-  @have "unique_keys_set (T - { KVPair k v })" @then
-  @have "\<forall>x. KVPair k x \<notin> T - { KVPair k v }"
+  @have "unique_keys_set (T - { (k, v) })" @then
+  @have "\<forall>x. (k, x) \<notin> T - { (k, v) }"
 @qed
 
 setup {* fold del_prfstep_thm [@{thm in_set_union_single}, @{thm member_union_single}] *}
 
-definition map_of_kv_list :: "('a, 'b) kv_pair list \<Rightarrow> ('a, 'b) map" where
+definition map_of_kv_list :: "('a \<times> 'b) list \<Rightarrow> ('a, 'b) map" where
   "map_of_kv_list xs = map_of_kv_set (set xs)"
 setup {* add_rewrite_rule @{thm map_of_kv_list_def} *}
 
@@ -279,18 +491,18 @@ partial_function (heap) idx_bubble_down ::
       vk \<leftarrow> idx_pqueue_nth a k;
       vs1k \<leftarrow> idx_pqueue_nth a (s1 k);
       vs2k \<leftarrow> idx_pqueue_nth a (s2 k);
-      (if vs1k \<le> vs2k then
-         if vk > vs1k then
+      (if snd vs1k \<le> snd vs2k then
+         if snd vk > snd vs1k then
            do { idx_pqueue_swap a k (s1 k); idx_bubble_down a (s1 k) }
          else return ()
        else
-         if vk > vs2k then
+         if snd vk > snd vs2k then
            do { idx_pqueue_swap a k (s2 k); idx_bubble_down a (s2 k) }
          else return ()) }
      else if s1 k < len then do {
        vk \<leftarrow> idx_pqueue_nth a k;
        vs1k \<leftarrow> idx_pqueue_nth a (s1 k);
-       (if vk > vs1k then
+       (if snd vk > snd vs1k then
           do { idx_pqueue_swap a k (s1 k); idx_bubble_down a (s1 k) }
         else return ()) }
      else return ()) }"
@@ -308,14 +520,15 @@ theorem idx_bubble_down_rule [hoare_triple]:
   @apply_induct_hyp "length xs - s2 k" @have "length xs - s2 k < length xs - k"
 @qed
 
-partial_function (heap) idx_bubble_up :: "'a::{heap,linorder} indexed_pqueue \<Rightarrow> nat \<Rightarrow> unit Heap" where
+partial_function (heap) idx_bubble_up ::
+  "'a::{heap,linorder} indexed_pqueue \<Rightarrow> nat \<Rightarrow> unit Heap" where
   "idx_bubble_up a k =
     (if k = 0 then return () else do {
        len \<leftarrow> idx_pqueue_length a;
        (if k < len then do {
           vk \<leftarrow> idx_pqueue_nth a k;
           vpk \<leftarrow> idx_pqueue_nth a (par k);
-          (if vk < vpk then
+          (if snd vk < snd vpk then
              do { idx_pqueue_swap a k (par k); idx_bubble_up a (par k) }
            else return ()) }
         else return ())})"
@@ -331,7 +544,7 @@ theorem idx_bubble_up_rule [hoare_triple]:
 @qed
 
 definition delete_min_idx_pqueue ::
-  "'a::{heap,linorder} indexed_pqueue \<Rightarrow> ((nat, 'a) kv_pair \<times> 'a indexed_pqueue) Heap" where
+  "'a::{heap,linorder} indexed_pqueue \<Rightarrow> ((nat \<times> 'a) \<times> 'a indexed_pqueue) Heap" where
   "delete_min_idx_pqueue p = do {
     len \<leftarrow> idx_pqueue_length p;
     (if len = 0 then raise ''delete_min''
@@ -351,14 +564,20 @@ theorem delete_min_idx_pqueue_rule [hoare_triple]:
 declare delete_min_idx_pqueue_def [sep_proc_defs del]
 
 setup {* add_rewrite_rule_back @{thm indexed_pqueue.collapse} *}
+setup {* add_rewrite_rule_cond @{thm surjective_pairing} [with_cond "?t \<noteq> (?a, ?b)"] *}
+lemma test1: "k = fst (k, v)" by simp
+setup {* add_forward_prfstep_cond @{thm test1} [with_term "(?k, ?v)"] *}
+lemma test2: "v = snd (k, v)" by simp
+setup {* add_forward_prfstep_cond @{thm test2} [with_term "(?k, ?v)"] *}
 
 theorem delete_min_idx_pqueue_map' [hoare_triple, hoare_create_case]:
   "<idx_pqueue xs p * \<up>(is_heap xs) * \<up>(length xs > 0)>
    delete_min_idx_pqueue p
-   <\<lambda>(x, r). \<exists>\<^sub>Axs'. idx_pqueue xs' r * \<up>(map_of_kv_list xs' = delete_map (key x) (map_of_kv_list xs))>"
+   <\<lambda>(x, r). \<exists>\<^sub>Axs'. idx_pqueue xs' r * \<up>(map_of_kv_list xs' = delete_map (fst x) (map_of_kv_list xs))>"
   by auto2
 
-definition insert_idx_pqueue :: "nat \<Rightarrow> 'a::{heap,linorder} \<Rightarrow> 'a indexed_pqueue \<Rightarrow> 'a indexed_pqueue Heap" where
+definition insert_idx_pqueue ::
+  "nat \<Rightarrow> 'a::{heap,linorder} \<Rightarrow> 'a indexed_pqueue \<Rightarrow> 'a indexed_pqueue Heap" where
   "insert_idx_pqueue k v p = do {
      p' \<leftarrow> idx_pqueue_push k v p;
      len \<leftarrow> idx_pqueue_length p';
@@ -372,15 +591,16 @@ theorem insert_idx_pqueue_rule [hoare_triple]:
    insert_idx_pqueue k v p
    <\<lambda>r. \<exists>\<^sub>Axs'. idx_pqueue xs' r * \<up>(is_heap xs') * \<up>(map_of_kv_list xs' = map_of_kv_list xs {k \<rightarrow> v})>\<^sub>t" by auto2
 
-definition update_idx_pqueue :: "nat \<Rightarrow> 'a::{heap,linorder} \<Rightarrow> 'a indexed_pqueue \<Rightarrow> unit Heap" where
+definition update_idx_pqueue ::
+  "nat \<Rightarrow> 'a::{heap,linorder} \<Rightarrow> 'a indexed_pqueue \<Rightarrow> unit Heap" where
   "update_idx_pqueue k v p = do {
     i_opt \<leftarrow> amap_lookup (index p) k;
     (case i_opt of
       None \<Rightarrow> raise ''update_idx_pqueue''
     | Some i \<Rightarrow> do {
         x \<leftarrow> array_nth (pqueue p) i;
-        array_upd i (KVPair k v) (pqueue p);
-        (if x \<le> KVPair k v then idx_bubble_down p i
+        array_upd i (k, v) (pqueue p);
+        (if snd x \<le> v then idx_bubble_down p i
          else idx_bubble_up p i) })
    }"
 declare update_idx_pqueue_def [sep_proc_defs]
@@ -395,8 +615,8 @@ theorem update_idx_pqueue_rule [hoare_triple]:
    <\<lambda>_. \<exists>\<^sub>Axs'. idx_pqueue xs' p * \<up>(is_heap xs') * \<up>(map_of_kv_list xs' = map_of_kv_list xs {k \<rightarrow> v})>"
 @proof
   @contradiction
-  @obtain v' where "KVPair k v' \<in># mset xs" @then
-  @obtain i where "i < length xs \<and> KVPair k v' = xs ! i"
+  @obtain v' where "(k, v') \<in># mset xs" @then
+  @obtain i where "i < length xs \<and> (k, v') = xs ! i"
 @qed
 setup {* del_prfstep_thm @{thm mset_update'} *}
 
@@ -407,10 +627,10 @@ definition idx_pqueue_map :: "(nat, 'a::{heap,linorder}) map \<Rightarrow> 'a in
 setup {* add_rewrite_ent_rule @{thm idx_pqueue_map_def} *}
 
 theorem has_key_set [rewrite]:
-  "has_key xs k \<longleftrightarrow> (\<exists>v. KVPair k v \<in> set xs)"
+  "has_key xs k \<longleftrightarrow> (\<exists>v. (k, v) \<in> set xs)"
 @proof
   @case "has_key xs k" @with
-    @obtain v where "KVPair k v \<in># mset xs" @then @have "KVPair k v \<in> set xs"
+    @obtain v where "(k, v) \<in># mset xs" @then @have "(k, v) \<in> set xs"
   @end
 @qed
 
@@ -419,19 +639,13 @@ theorem has_key_to_map_none [rewrite_bidir]:
 setup {* del_prfstep_thm @{thm has_key_set} *}
 
 theorem heap_implies_hd_min2 [backward1]:
-  "is_heap xs \<Longrightarrow> xs \<noteq> [] \<Longrightarrow> (map_of_kv_list xs)\<langle>k\<rangle> = Some v \<Longrightarrow> val (hd xs) \<le> v"
+  "is_heap xs \<Longrightarrow> xs \<noteq> [] \<Longrightarrow> (map_of_kv_list xs)\<langle>k\<rangle> = Some v \<Longrightarrow> snd (hd xs) \<le> v"
 @proof
-  @obtain i where "i < length xs \<and> KVPair k v = xs ! i" @with @have "KVPair k v \<in> set xs" @end
-  @have "hd xs \<le> KVPair k v"
+  @obtain i where "i < length xs \<and> (k, v) = xs ! i" @with @have "(k, v) \<in> set xs" @end
 @qed
 
 theorem empty_list_to_empty_map [rewrite]:
-  "map_of_kv_list ([]::('a, 'b) kv_pair list) = empty_map"
-@proof
-  @contradiction
-  @obtain x where "(map_of_kv_list ([]::('a, 'b) kv_pair list))\<langle>x\<rangle> \<noteq> None" @then
-  @obtain v where "KVPair x v \<in> set ([]::('a, 'b) kv_pair list)"
-@qed
+  "map_of_kv_list ([]::('a \<times> 'b) list) = empty_map" by auto2
 
 declare idx_pqueue_empty_def [sep_proc_defs del]
 theorem idx_pqueue_empty_map:
@@ -443,7 +657,7 @@ declare delete_min_idx_pqueue_def [sep_proc_defs del]
 theorem delete_min_idx_pqueue_map:
   "<idx_pqueue_map M p * \<up>(M \<noteq> empty_map)>
    delete_min_idx_pqueue p
-   <\<lambda>(x, r). idx_pqueue_map (delete_map (key x) M) r * \<up>(\<forall>k v. M\<langle>k\<rangle> = Some v \<longrightarrow> val x \<le> v)>"
+   <\<lambda>(x, r). idx_pqueue_map (delete_map (fst x) M) r * \<up>(\<forall>k v. M\<langle>k\<rangle> = Some v \<longrightarrow> snd x \<le> v)>"
   by auto2
 
 declare insert_idx_pqueue_def [sep_proc_defs del]
